src/Distributions/UniformPowerOfTwo/Implementation.dfy
@@ -7,13 +7,13 @@ include "Interface.dfy"
 include "Model.dfy"
 
 module UniformPowerOfTwoImplementation {
-  import UniformPowerOfTwoModel
-  import UniformPowerOfTwoInterface
+  import Model = UniformPowerOfTwoModel
+  import Interface = UniformPowerOfTwoInterface
 
-  trait {:termination false} TUniformPowerOfTwo extends UniformPowerOfTwoInterface.IUniformPowerOfTwo {
-    method UniformPowerOfTwo(n: nat) returns (u: nat)
+  trait {:termination false} Trait extends Interface.Trait {
+    method UniformPowerOfTwoSample(n: nat) returns (u: nat)
       modifies this
-      ensures UniformPowerOfTwoModel.UnifModel(n)(old(s)) == (u, s)
+      ensures Model.UnifModel(n)(old(s)) == (u, s)
     {
       var k := 1;
       u := 0;
@@ -21,9 +21,9 @@ module UniformPowerOfTwoImplementation {
       while k <= n
         decreases 2*n - k
         invariant k >= 1
-        invariant UniformPowerOfTwoModel.UnifAlternativeModel(n)(old(s)) == UniformPowerOfTwoModel.UnifAlternativeModel(n, k, u)(s)
+        invariant Model.UnifAlternativeModel(n)(old(s)) == Model.UnifAlternativeModel(n, k, u)(s)
       {
-        var b := Coin();
+        var b := CoinSample();
         k := 2*k;
         u := if b then 2*u + 1 else 2*u;
       }
