src/Distributions/BernoulliExpNeg/BernoulliExpNeg.dfy
@@ -1,0 +1,7 @@
+include "Interface.dfy"
+include "Implementation.dfy"
+
+module BernoulliExpNeg {
+  import Interface = BernoulliExpNegInterface
+  import Implementation = BernoulliExpNegImplementation
+}
