src/Distributions/BernoulliExpNeg/Implementation.dfy
@@ -4,41 +4,40 @@
  *******************************************************************************/
 
 include "../../Math/Rationals.dfy"
-include "../Bernoulli/Interface.dfy"
 include "Interface.dfy"
 
 module BernoulliExpNegImplementation {
   import Rationals
-  import BernoulliExpNegInterface
+  import Interface = BernoulliExpNegInterface
 
-  trait {:termination false} TBernoulliExpNeg extends BernoulliExpNegInterface.IBernoulliExpNeg {
+  trait {:termination false} Trait extends Interface.Trait {
 
     // Based on Algorithm 1 in https://arxiv.org/pdf/2004.00010.pdf; unverified
-    method BernoulliExpNeg(gamma: Rationals.Rational) returns (c: bool)
+    method BernoulliExpNegSample(gamma: Rationals.Rational) returns (c: bool)
       modifies this
       requires gamma.numer >= 0
       decreases *
     {
       if gamma.numer <= gamma.denom {
         var k := 1;
-        var a := Bernoulli(Rationals.Rational(gamma.numer, k * gamma.denom));
+        var a := BernoulliSample(Rationals.Rational(gamma.numer, k * gamma.denom));
         while a
           decreases *
         {
           k := k + 1;
-          a := Bernoulli(Rationals.Rational(gamma.numer, k * gamma.denom));
+          a := BernoulliSample(Rationals.Rational(gamma.numer, k * gamma.denom));
         }
         c := k % 2 == 1;
       } else {
         var k := 1;
         while k <= Rationals.Floor(gamma) {
-          var b := BernoulliExpNeg(Rationals.Int(1));
+          var b := BernoulliExpNegSample(Rationals.Int(1));
           if !b {
             return false;
           }
           k := k + 1;
         }
-        c:= BernoulliExpNeg(Rationals.FractionalPart(gamma));
+        c:= BernoulliExpNegSample(Rationals.FractionalPart(gamma));
       }
     }
 
