src/Distributions/DiscreteGaussian/DiscreteGaussian.dfy
@@ -1,0 +1,7 @@
+include "Implementation.dfy"
+include "Interface.dfy"
+
+module DiscreteGaussian {
+  import Interface = DiscreteGaussianInterface
+  import Implementation = DiscreteGaussianImplementation
+}
