src/Distributions/DiscreteLaplace/DiscreteLaplace.dfy
@@ -1,0 +1,7 @@
+include "Implementation.dfy"
+include "Interface.dfy"
+
+module DiscreteLaplace {
+  import Interface = DiscreteLaplaceInterface
+  import Implementation = DiscreteLaplaceImplementation
+}
